theories/State.v
@@ -378,6 +378,22 @@ Fixpoint show_expr (e : Expr) : PrimString.string :=
               (PrimString.cat (show_expr c) ")")))))
   | EBool b => if b then "TRUE" else "FALSE"
   | EBNot a => PrimString.cat "BNOT(" (PrimString.cat (show_expr a) ")")
+  | EUpper a => PrimString.cat "UPPER(" (PrimString.cat (show_expr a) ")")
+  | ELower a => PrimString.cat "LOWER(" (PrimString.cat (show_expr a) ")")
+  | ETrim a => PrimString.cat "TRIM(" (PrimString.cat (show_expr a) ")")
+  | EFind a b => PrimString.cat "FIND("
+                  (PrimString.cat (show_expr a)
+                    (PrimString.cat ","
+                      (PrimString.cat (show_expr b) ")")))
+  | EReplaceS a b c d =>
+    PrimString.cat "REPLACE("
+      (PrimString.cat (show_expr a)
+        (PrimString.cat ","
+          (PrimString.cat (show_expr b)
+            (PrimString.cat ","
+              (PrimString.cat (show_expr c)
+                (PrimString.cat ","
+                  (PrimString.cat (show_expr d) ")")))))))
   | EBAnd a b => PrimString.cat "BAND("
                   (PrimString.cat (show_expr a)
                     (PrimString.cat ","
